updates

src/Distributions/DiscreteLaplace/Correctness.dfy
@@ -15,26 +15,26 @@ module DiscreteLaplace.Correctness {
   ghost function Numerator1(scale: Rationals.Rational): real
     requires scale.numer >= 1
   {
-    Exponential.Exp((1.0 / Rationals.ToReal(scale)) - 1.0)
+    Exponential.Exp((1.0 / scale.ToReal()) - 1.0)
   }
 
   ghost function Numerator2(scale: Rationals.Rational, x: int): real
     requires scale.numer >= 1
   {
-    Exponential.Exp(-((RealArith.Abs(x as real)) / Rationals.ToReal(scale)))
+    Exponential.Exp(-((RealArith.Abs(x as real)) / scale.ToReal()))
   }
 
   ghost function Denominator(scale: Rationals.Rational): (r: real)
     requires scale.numer >= 1
     ensures r > 0.0
   {
-    var x := (1.0 / Rationals.ToReal(scale)) + 1.0;
+    var x := (1.0 / scale.ToReal()) + 1.0;
     Exponential.Positive(x);
     Exponential.Exp(x)
   }
 
   lemma {:axiom} Correctness(scale: Rationals.Rational, x: int)
     requires scale.numer >= 1
-    ensures Rand.prob(iset s | Model.Sample(scale)(s).value == x) == (Numerator1(scale) * Numerator2(scale, x)) / Denominator(scale)
+    ensures Rand.prob(iset s | Model.Sample(scale)(s).Equals(x)) == (Numerator1(scale) * Numerator2(scale, x)) / Denominator(scale)
 
 }
