src/Distributions/DiscreteLaplace/Model.dfy
@@ -10,6 +10,7 @@ module DiscreteLaplace.Model {
   import Uniform
   import BernoulliExpNeg
   import Bernoulli
+  import Coin
 
   ghost function Sample(scale: Rationals.Rational): Monad.Hurd<int>
     requires scale.numer >= 1
@@ -25,16 +26,30 @@ module DiscreteLaplace.Model {
       if !(b && y == 0) then
         Monad.Result(if b then -y else y, s)
       else
-        var (u, s) := Monad.Extract(Uniform.Model.Sample(scale.numer)(s));
-        var (d, s) := Monad.Extract(BernoulliExpNeg.Model.Sample(Rationals.Rational(u, scale.numer))(s));
-        if !d then
-          SampleTailRecursive(scale, b, y)(s)
+        var sample := Uniform.Model.Sample(scale.numer)(s);
+        if sample.Result? then
+          var (u, s) := (sample.value, sample.rest);
+          var sample := BernoulliExpNeg.Model.Sample(Rationals.Rational(u, scale.numer))(s);
+          if sample.Result? then
+            var (d, s) := (sample.value, sample.rest);
+            if !d then
+              SampleTailRecursive(scale, b, y)(s)
+            else
+              var sample := SampleTailRecursiveHelper(scale)(s);
+              if sample.Result? then
+                var (v, s) := (sample.value, sample.rest);
+                var x := u + scale.numer * v;
+                var y := x / scale.denom;
+                var sample := Coin.Model.Sample(s);
+                var (b, s) := (sample.value, sample.rest);
+                SampleTailRecursive(scale, b, y)(s)
+              else
+                Monad.Diverging
+          else
+            Monad.Diverging
         else
-          var (v, s) := Monad.Extract(SampleTailRecursiveHelper(scale)(s));
-          var x := u + scale.numer * v;
-          var y := x / scale.denom;
-          var (b, s) := Monad.Extract(Bernoulli.Model.Sample(1, 2)(s));
-          SampleTailRecursive(scale, b, y)(s)
+          Monad.Diverging
+
   }
 
   ghost function SampleTailRecursiveHelper(scale: Rationals.Rational, v: int := 0, a: bool := true): Monad.Hurd<int> {
@@ -43,8 +58,12 @@ module DiscreteLaplace.Model {
       if !a then
         Monad.Result(v, s)
       else
-        var (a, s) := Monad.Extract(BernoulliExpNeg.Model.Sample(Rationals.Int(1))(s));
-        SampleTailRecursiveHelper(scale, if a then v + 1 else v, a)(s)
+        var sample := BernoulliExpNeg.Model.Sample(Rationals.Int(1))(s);
+        if sample.Result? then
+          var (a, s) := (sample.value, sample.rest);
+          SampleTailRecursiveHelper(scale, if a then v + 1 else v, a)(s)
+        else
+          Monad.Diverging
   }
 
 }
